# baseURI: http://www.opengis.net/def/netcdf
# imports: http://www.opengis.net/def/ogc-na



@prefix dc:      <http://purl.org/dc/elements/1.1/> .
@prefix dct:     <http://purl.org/dc/terms/> .
@prefix netcdf:  <http://www.opengis.net/def/netcdf/> .
@prefix owl:     <http://www.w3.org/2002/07/owl#> .
@prefix policy:  <http://www.opengis.net/ogc-na#> .
@prefix rdf:     <http://www.w3.org/1999/02/22-rdf-syntax-ns#> .
@prefix rdfs:    <http://www.w3.org/2000/01/rdf-schema#> .
@prefix skos:    <http://www.w3.org/2004/02/skos/core#> .
@prefix xsd:     <http://www.w3.org/2001/XMLSchema#> .
@prefix status: <http://www.opengis.net/def/status/> .


<http://www.opengis.net/def/ogc-netcdf>
      rdf:type skos:ConceptScheme ;
      rdfs:label "OGC NetCDF definitions" ;
      skos:prefLabel "OGC NetCDF definitions" .

<http://www.opengis.net/def/netcdf>
      rdf:type owl:Ontology ;
      rdfs:comment "Definitions from OGC netCDF standards"^^xsd:string ;
      rdfs:seeAlso <http://www.opengeospatial.org/standards/netcdf> , <http://www.opengis.net/def/property/netcdf/> ;
      owl:imports <http://www.opengis.net/def/ogc-na> ;
      owl:versionIRI <https://svn.opengeospatial.org/ogc-projects/sp/ogc-na/tags/2012-10/definitions/netcdf.rdf> .

<http://www.opengis.net/def/property>
      skos:member <http://www.opengis.net/def/property/netcdf/> .

<http://www.opengis.net/def/property/>
      skos:member <http://www.opengis.net/def/property/netcdf/> .

<http://www.opengis.net/def/property/netcdf>
      owl:sameAs <http://www.opengis.net/def/property/netcdf/> .

<http://www.opengis.net/def/property/netcdf/>
      rdf:type skos:Collection ;
      rdfs:label "netCDF properties" ;
      skos:member <http://www.opengis.net/def/property/netcdf/1.0/> .

<http://www.opengis.net/def/property/netcdf/1.0>
      rdfs:label ""^^xsd:string ;
      owl:sameAs <http://www.opengis.net/def/property/netcdf/1.0/> ;
      skos:prefLabel ""^^xsd:string .

<http://www.opengis.net/def/property/netcdf/1.0/>
      rdf:type skos:Collection ;
      rdfs:label "netCDF properties 1.0" ;
      skos:member <http://www.opengis.net/def/property/netcdf/1.0/compoundType> , <http://www.opengis.net/def/property/netcdf/1.0/string> , <http://www.opengis.net/def/property/netcdf/1.0/unsignedInt64> , <http://www.opengis.net/def/property/netcdf/1.0/int> , <http://www.opengis.net/def/property/netcdf/1.0/short> , <http://www.opengis.net/def/property/netcdf/1.0/char> , <http://www.opengis.net/def/property/netcdf/1.0/group> , <http://www.opengis.net/def/property/netcdf/1.0/byte> , <http://www.opengis.net/def/property/netcdf/1.0/enumeratedType> , <http://www.opengis.net/def/property/netcdf/1.0/opaqueType> , <http://www.opengis.net/def/property/netcdf/1.0/float> , <http://www.opengis.net/def/property/netcdf/1.0/long> , <http://www.opengis.net/def/property/netcdf/1.0/int64> , <http://www.opengis.net/def/property/netcdf/1.0/unsignedShort> , <http://www.opengis.net/def/property/netcdf/1.0/unsignedInt> , <http://www.opengis.net/def/property/netcdf/1.0/real> , <http://www.opengis.net/def/property/netcdf/1.0/variableLengthType> , <http://www.opengis.net/def/property/netcdf/1.0/double> , <http://www.opengis.net/def/property/netcdf/1.0/userDefinedType> .

<http://www.opengis.net/def/property/netcdf/1.0/byte>
      rdf:type skos:Concept ;
      rdfs:label "byte"^^xsd:string , "byte"@en ;
      rdfs:seeAlso <http://www.opengis.net/doc/netcdf/1.0#clause-4.1> , "OGC netCDF Clause 4.1"^^xsd:string , <http://www.opengis.net/doc/netcdf#clause-4.1> ;
      dc:source <http://www.opengis.net/doc/netcdf#clause-4.1> , "OGC netCDF Clause 4.1"^^xsd:string ;
      dct:created "2012-03-27"^^xsd:date ;
      policy:status status:valid ;
      skos:definition "A byte is an eight-bit integer.  The byte type differs from the char type in that it is intended for eight-bit data, and the zero byte has no special significance, as it may for character data."^^xsd:string ;
      skos:inScheme <http://www.opengis.net/def/scheme> ;
      skos:prefLabel "byte"@en .

<http://www.opengis.net/def/property/netcdf/1.0/char>
      rdf:type skos:Concept ;
      rdfs:label "character"^^xsd:string , "character"@en ;
      rdfs:seeAlso "OGC netCDF Clause 4.2"^^xsd:string , <http://www.opengis.net/doc/netcdf/1.0#clause-4.2> , <http://www.opengis.net/doc/netcdf#clause-4.2> ;
      dc:source "OGC netCDF Clause 4.2"^^xsd:string , <http://www.opengis.net/doc/netcdf#clause-4.2> ;
      policy:status status:valid ;
      skos:definition "A char is a single Unicode character, and may use up to 32 bits. (Note that ASCII characters are represented in Unicode using 8 bits.)"^^xsd:string ;
      skos:inScheme <http://www.opengis.net/def/scheme> ;
      skos:prefLabel "character"@en .

<http://www.opengis.net/def/property/netcdf/1.0/compound-type>
      rdf:type skos:Concept ;
      policy:status status:valid .

<http://www.opengis.net/def/property/netcdf/1.0/compoundType>
      rdf:type skos:Concept ;
      rdfs:label "compound type"^^xsd:string , "compound type"@en ;
      rdfs:seeAlso "OGC netCDF Clause 4.3"^^xsd:string , <http://www.opengis.net/doc/netcdf/1.0#clause-4.3> , <http://www.opengis.net/doc/netcdf#clause-4.3> ;
      dc:source "OGC netCDF Clause 4.3"^^xsd:string , <http://www.opengis.net/doc/netcdf#clause-4.3> ;
      policy:status status:valid ;
      owl:sameAs <http://www.opengis.net/def/property/netcdf/1.0/compound-type> ;
      skos:definition """Compound types are like C structures, grouping together named fields (also called \"members\"), that may be of different types, into a structure that may be accessed as a unit. It has a fixed total size. It consists of zero or more named members that do not overlap with other members.

    Each member has a name distinct from other members.
    Each member has its own datatype.
    Each member is referenced by an index number between zero and N-1, where N is the number of members in the compound datatype.
    Each member has a fixed byte offset, which is the first byte (smallest byte address) of that member in the compound datatype.
    In addition to other other user-defined data types or atomic datatypes, a member can be a small fixed-size array of any type with up to four fixed-size “dimensions” (not associated with named netCDF dimensions)."""^^xsd:string ;
      skos:inScheme <http://www.opengis.net/def/scheme> ;
      skos:prefLabel "compound type"@en .

<http://www.opengis.net/def/property/netcdf/1.0/double>
      rdf:type skos:Concept ;
      rdfs:label "Double-precision floating point number"@en , "Double-precision floating point number"^^xsd:string ;
      rdfs:seeAlso <http://www.opengis.net/doc/netcdf#clause-4.4> , <http://www.opengis.net/doc/netcdf/1.0#clause-4.4> , "OGC netCDF Clause 4.4"^^xsd:string ;
      dc:source "OGC netCDF Clause 4.4"^^xsd:string , <http://www.opengis.net/doc/netcdf#clause-4.4> ;
      policy:status status:valid ;
      skos:definition "A double is an IEEE double-precision floating point (64 bits.).  The double type can hold values between about -1.7+308 and 1.7+308, with external representation as 64-bit IEEE standard normalized double-precision, floating-point numbers"^^xsd:string ;
      skos:inScheme <http://www.opengis.net/def/scheme> ;
      skos:prefLabel "Double-precision floating point number"@en .

<http://www.opengis.net/def/property/netcdf/1.0/enumerated-type>
      rdf:type skos:Concept ;
      policy:status status:valid .

<http://www.opengis.net/def/property/netcdf/1.0/enumeratedType>
      rdf:type skos:Concept ;
      rdfs:label "Enumeration"^^xsd:string , "Enumeration"@en ;
      rdfs:seeAlso "OGC netCDF Clause 4.5"^^xsd:string , <http://www.opengis.net/doc/netcdf/1.0#clause-4.5> , <http://www.opengis.net/doc/netcdf#clause-4.5> ;
      dc:source "OGC netCDF Clause 4.5"^^xsd:string , <http://www.opengis.net/doc/netcdf#clause-4.5> ;
      policy:status status:valid ;
      owl:sameAs <http://www.opengis.net/def/property/netcdf/1.0/enumerated-type> ;
      skos:definition "Enumerated types are used to represent a small number of named values more concisely than strings"^^xsd:string ;
      skos:inScheme <http://www.opengis.net/def/scheme> ;
      skos:prefLabel "Enumeration"@en .

<http://www.opengis.net/def/property/netcdf/1.0/float>
      rdf:type skos:Concept ;
      rdfs:label "Single-precision floating point number"@en , "Single-precision floating point number"^^xsd:string ;
      rdfs:seeAlso <http://www.opengis.net/doc/netcdf/1.0#clause-4.6> , "OGC netCDF Clause 4.6"^^xsd:string , <http://www.opengis.net/doc/netcdf#clause-4.6> ;
      dc:source <http://www.opengis.net/doc/netcdf#clause-4.6> , "OGC netCDF Clause 4.6"^^xsd:string ;
      policy:status status:valid ;
      skos:definition "A float is an IEEE single-precision floating point (32 bits).  The float type can hold values between about -3.4+38 and 3.4+38, with external representation as 32-bit IEEE normalized single-precision floating-point numbers"^^xsd:string ;
      skos:inScheme <http://www.opengis.net/def/scheme> ;
      skos:prefLabel "Single-precision floating point number"@en .

<http://www.opengis.net/def/property/netcdf/1.0/group>
      rdf:type skos:Concept ;
      rdfs:label "Group"^^xsd:string ;
      rdfs:seeAlso <http://www.opengis.net/doc/netcdf#clause-4.7> , <http://www.opengis.net/doc/netcdf/1.0#clause-4.7> , "OGC netCDF Clause 4.7"^^xsd:string ;
      dc:source <http://www.opengis.net/doc/netcdf#clause-4.7> , "OGC netCDF Clause 4.7"^^xsd:string ;
      policy:status status:valid ;
      skos:definition "A group provides a nested scope for names"^^xsd:string ;
      skos:inScheme <http://www.opengis.net/def/scheme> ;
      skos:prefLabel "Group"@en .

<http://www.opengis.net/def/property/netcdf/1.0/int>
      rdf:type skos:Concept ;
      rdfs:label "32-bit signed integer"@en , "32-bit signed integer"^^xsd:string ;
      rdfs:seeAlso "OGC netCDF Clause 4.8"^^xsd:string , <http://www.opengis.net/doc/netcdf/1.0#clause-4.8> , <http://www.opengis.net/doc/netcdf#clause-4.8> ;
      dc:source <http://www.opengis.net/doc/netcdf#clause-4.8> , "OGC netCDF Clause 4.8"^^xsd:string ;
      policy:status status:valid ;
      skos:definition "An int is a 32-bit signed integer.  An int can hold values between -2147483648 and 2147483647"^^xsd:string ;
      skos:inScheme <http://www.opengis.net/def/scheme> ;
      skos:prefLabel "32-bit signed integer"@en .

<http://www.opengis.net/def/property/netcdf/1.0/int64>
      rdf:type skos:Concept ;
      rdfs:label "8-byte signed integer"^^xsd:string , "8-byte signed integer"@en ;
      rdfs:seeAlso "OGC netCDF Clause 4.9"^^xsd:string , <http://www.opengis.net/doc/netcdf/1.0#clause-4.9> , <http://www.opengis.net/doc/netcdf#clause-4.9> ;
      dc:source <http://www.opengis.net/doc/netcdf#clause-4.9> , "OGC netCDF Clause 4.9"^^xsd:string ;
      policy:status status:valid ;
      skos:definition "An int64 is an eight-byte signed integer.   An int64 can hold values between -9223372036854775808 and 9223372036854775807"^^xsd:string ;
      skos:inScheme <http://www.opengis.net/def/scheme> ;
      skos:prefLabel "8-byte signed integer"@en .

<http://www.opengis.net/def/property/netcdf/1.0/long>
      rdf:type skos:Concept ;
      rdfs:label "Long integer"^^xsd:string , "Long integer"@en ;
      rdfs:seeAlso <http://www.opengis.net/doc/netcdf#clause-4.10> , <http://www.opengis.net/doc/netcdf/1.0#clause-4.10> , "OGC netCDF Clause 4.10"^^xsd:string ;
      dc:source "OGC netCDF Clause 4.10"^^xsd:string , <http://www.opengis.net/doc/netcdf#clause-4.10> ;
      policy:status status:valid ;
      skos:definition "The long type is deprecated.  It is synonymous with int"^^xsd:string ;
      skos:inScheme <http://www.opengis.net/def/scheme> ;
      skos:prefLabel "Long integer"@en .

<http://www.opengis.net/def/property/netcdf/1.0/opaque-type>
      rdf:type skos:Concept ;
      policy:status status:valid ;
      owl:sameAs <http://www.opengis.net/def/property/netcdf/1.0/opaqueType> .

<http://www.opengis.net/def/property/netcdf/1.0/opaqueType>
      rdf:type skos:Concept ;
      rdfs:label "Opaque collection"^^xsd:string , "Opaque collection"@en ;
      rdfs:seeAlso <http://www.opengis.net/doc/netcdf/1.0#clause-4.11> , <http://www.opengis.net/doc/netcdf#clause-4.11> , "OGC netCDF Clause 4.11"^^xsd:string ;
      dc:source "OGC netCDF Clause 4.11"^^xsd:string , <http://www.opengis.net/doc/netcdf#clause-4.11> ;
      policy:status status:valid ;
      owl:sameAs <http://www.opengis.net/def/property/netcdf/1.0/opaque-type> ;
      skos:definition "Opaque is a collection of objects of a known size.  Each object is the same size.  Nothing is known to netCDF about the contents of these blobs of data, except their size in bytes, and the name of the type"^^xsd:string ;
      skos:inScheme <http://www.opengis.net/def/scheme> ;
      skos:prefLabel "Opaque collection"@en .

<http://www.opengis.net/def/property/netcdf/1.0/real>
      rdf:type skos:Concept ;
      rdfs:label "Real number"^^xsd:string , "Real number"@en ;
      rdfs:seeAlso <http://www.opengis.net/doc/netcdf/1.0#clause-4.12> , <http://www.opengis.net/doc/netcdf#clause-4.12> , "OGC netCDF Clause 4.12"^^xsd:string ;
      dc:source "OGC netCDF Clause 4.12"^^xsd:string , <http://www.opengis.net/doc/netcdf#clause-4.12> ;
      policy:status status:valid ;
      skos:definition "The real type is synonymous with float"^^xsd:string ;
      skos:inScheme <http://www.opengis.net/def/scheme> ;
      skos:prefLabel "Real number"@en .

<http://www.opengis.net/def/property/netcdf/1.0/short>
      rdf:type skos:Concept ;
      rdfs:label "Short integer"@en , "Short integer"^^xsd:string ;
      rdfs:seeAlso <http://www.opengis.net/doc/netcdf/1.0#clause-4.13> , <http://www.opengis.net/doc/netcdf#clause-4.13> , "OGC netCDF Clause 4.13"^^xsd:string ;
      dc:source "OGC netCDF Clause 4.13"^^xsd:string , <http://www.opengis.net/doc/netcdf#clause-4.13> ;
      policy:status status:valid ;
      skos:definition "A short is a 16-bit signed integer.  A short holds values between -32768 and 32767"^^xsd:string ;
      skos:inScheme <http://www.opengis.net/def/scheme> ;
      skos:prefLabel "Short integer"@en .

<http://www.opengis.net/def/property/netcdf/1.0/string>
      rdf:type skos:Concept ;
      rdfs:label "Character string"^^xsd:string , "Character string"@en ;
      rdfs:seeAlso "OGC netCDF Clause 4.14"^^xsd:string , <http://www.opengis.net/doc/netcdf/1.0#clause-4.14> , <http://www.opengis.net/doc/netcdf#clause-4.14> ;
      dc:source <http://www.opengis.net/doc/netcdf#clause-4.14> , "OGC netCDF Clause 4.14"^^xsd:string ;
      policy:status status:valid ;
      skos:definition "A string is a variable length string of characters"^^xsd:string ;
      skos:inScheme <http://www.opengis.net/def/scheme> ;
      skos:prefLabel "Character string"@en .

<http://www.opengis.net/def/property/netcdf/1.0/unsigned-int>
      rdf:type skos:Concept ;
      policy:status status:valid ;
      owl:sameAs <http://www.opengis.net/def/property/netcdf/1.0/unsignedInt> .

<http://www.opengis.net/def/property/netcdf/1.0/unsigned-int-64>
      rdf:type skos:Concept ;
      policy:status status:valid ;
      owl:sameAs <http://www.opengis.net/def/property/netcdf/1.0/unsignedInt64> .

<http://www.opengis.net/def/property/netcdf/1.0/unsigned-short>
      rdf:type skos:Concept ;
      policy:status status:valid ;
      owl:sameAs <http://www.opengis.net/def/property/netcdf/1.0/unsignedShort> .

<http://www.opengis.net/def/property/netcdf/1.0/unsignedInt>
      rdf:type skos:Concept ;
      rdfs:label "Unsigned 32-bit Integer"@en , "Unsigned 32-bit Integer"^^xsd:string ;
      rdfs:seeAlso <http://www.opengis.net/doc/netcdf/1.0#clause-4.15> , "OGC netCDF Clause 4.15"^^xsd:string , <http://www.opengis.net/doc/netcdf#clause-4.15> ;
      dc:source "OGC netCDF Clause 4.15"^^xsd:string , <http://www.opengis.net/doc/netcdf#clause-4.15> ;
      policy:status status:valid ;
      owl:sameAs <http://www.opengis.net/def/property/netcdf/1.0/unsigned-int> ;
      skos:definition "An unsigned int is a 32-bit unsigned integer.  An unsigned int holds values between 0 and 4294967296"^^xsd:string ;
      skos:inScheme <http://www.opengis.net/def/scheme> ;
      skos:prefLabel "Unsigned 32-bit Integer"@en .

<http://www.opengis.net/def/property/netcdf/1.0/unsignedInt64>
      rdf:type skos:Concept ;
      rdfs:label "Unsigned 64-bit Integer"@en , "Unsigned 64-bit Integer"^^xsd:string ;
      rdfs:seeAlso <http://www.opengis.net/doc/netcdf#clause-4.16> , <http://www.opengis.net/doc/netcdf/1.0#clause-4.16> , "OGC netCDF Clause 4.16"^^xsd:string ;
      dc:source "OGC netCDF Clause 4.16"^^xsd:string , <http://www.opengis.net/doc/netcdf#clause-4.16> ;
      policy:status status:valid ;
      owl:sameAs <http://www.opengis.net/def/property/netcdf/1.0/unsigned-int-64> ;
      skos:definition "An unsigned int64 is an unsigned 8-byte integer type. An unsigned int64 can hold values between 0 and 18446744073709551616"^^xsd:string ;
      skos:inScheme <http://www.opengis.net/def/scheme> ;
      skos:prefLabel "Unsigned 64-bit Integer"@en .

<http://www.opengis.net/def/property/netcdf/1.0/unsignedShort>
      rdf:type skos:Concept ;
      rdfs:label "Unsigned Short"^^xsd:string ;
      rdfs:seeAlso <http://www.opengis.net/doc/netcdf#clause-4.17> , "OGC netCDF Clause 4.17"^^xsd:string , <http://www.opengis.net/doc/netcdf/1.0#clause-4.17> ;
      dc:source "OGC netCDF Clause 4.17"^^xsd:string , <http://www.opengis.net/doc/netcdf#clause-4.17> ;
      policy:status status:valid ;
      owl:sameAs <http://www.opengis.net/def/property/netcdf/1.0/unsigned-short> ;
      skos:definition "An unsigned short is a 16-bit unsigned integer.  An unsigned short holds values between 0 and 65536"^^xsd:string ;
      skos:inScheme <http://www.opengis.net/def/scheme> ;
      skos:prefLabel "Unsigned Short"@en .

<http://www.opengis.net/def/property/netcdf/1.0/user-defined-type>
      rdf:type skos:Concept ;
      policy:status status:valid ;
      owl:sameAs <http://www.opengis.net/def/property/netcdf/1.0/userDefinedType> .

<http://www.opengis.net/def/property/netcdf/1.0/userDefinedType>
      rdf:type skos:Concept ;
      rdfs:label "User Defined Type"^^xsd:string , "User Defined Type"@en ;
      rdfs:seeAlso "OGC netCDF Clause 4.18"^^xsd:string , <http://www.opengis.net/doc/netcdf/1.0#clause-4.18> , <http://www.opengis.net/doc/netcdf#clause-4.18> ;
      dc:source <http://www.opengis.net/doc/netcdf#clause-4.18> , "OGC netCDF Clause 4.18"^^xsd:string ;
      policy:status status:valid ;
      owl:sameAs <http://www.opengis.net/def/property/netcdf/1.0/user-defined-type> ;
      skos:definition "User defined types are: compound, enumerated, variable-length, and opaque"^^xsd:string ;
      skos:inScheme <http://www.opengis.net/def/scheme> ;
      skos:prefLabel "User Defined Type"@en .

<http://www.opengis.net/def/property/netcdf/1.0/variable-length-type>
      rdf:type skos:Concept ;
      policy:status status:valid ;
      owl:sameAs <http://www.opengis.net/def/property/netcdf/1.0/variableLengthType> .

<http://www.opengis.net/def/property/netcdf/1.0/variableLengthType>
      rdf:type skos:Concept ;
      rdfs:label "Variable Length Type"^^xsd:string , "Variable Length Type"@en ;
      rdfs:seeAlso "OGC netCDF Clause 4.19"^^xsd:string , <http://www.opengis.net/doc/netcdf/1.0#clause-4.19> , <http://www.opengis.net/doc/netcdf#clause-4.19> ;
      dc:source <http://www.opengis.net/doc/netcdf#clause-4.19> , "OGC netCDF Clause 4.19"^^xsd:string ;
      policy:status status:valid ;
      owl:sameAs <http://www.opengis.net/def/property/netcdf/1.0/variable-length-type> ;
      skos:definition "The variable length type represents a one-dimensional array of variable length"^^xsd:string ;
      skos:inScheme <http://www.opengis.net/def/scheme> ;
      skos:prefLabel "Variable Length Type"@en .
